

$$g(x) = (|x| + |4x - 7|) \underbrace{([x^2] - 3)}$$

$$\boxed{0, 1, \sqrt{2}, \sqrt{3}}$$

$$\frac{-3(|x| + \cancel{7} - 4x) + \cancel{2}}{x}$$

$x \rightarrow 0$

$$3 \left(4 - \frac{|x|}{x} \right)$$

$$x \rightarrow \frac{7}{4} \quad \frac{0}{x - 7/4} = 0$$

$$\left(-\frac{1}{2}, 2\right)$$

$$\rightarrow -3$$

$$\rightarrow -2$$

$$\rightarrow -1$$

$$0$$

$$\left(-\frac{1}{2}, 1\right)$$

$$x \in [1, \sqrt{2})$$

$$x \in [\sqrt{2}, \sqrt{3})$$

$$x \in [\sqrt{3}, 2)$$

$$y=0$$

$$f(x) = f(x)f'(0) + f'(x)$$

$$\frac{1}{2}f(x) = f'(x)$$

$$\frac{dy}{dx} = \frac{1}{2}y$$

$$\int \frac{dy}{y} = \frac{1}{2} \int dx$$

$$\ln y = \frac{1}{2}x + C \rightarrow 0$$

$$f'(0) = \frac{1}{2}$$

$$f(0) = 2f(0)f'(0)$$

$$\int \frac{dy}{y+1} = \int dx$$

$$\ln(y+1) = x + C$$

$$f(x) = e^{x-1} (x^2 + \sin x) g(x) - 0$$

$$\lim_{x \rightarrow 1}$$

$$\lim_{x \rightarrow 0} \frac{0}{x}$$

$$= 0$$

$$f'(x) = (f(x)+1) \left(\lim_{h \rightarrow 0} \frac{f(h)}{h} \right)$$

$$f'(x) = (f(x)+1) f'(0) = f(x)+1$$

$$f'(0) = \lim_{x \rightarrow 0} \frac{f(x)-f(0)}{x-0} = 1$$

$$(13) \quad u g(x) = e^x - 1$$

$$g(x) = \frac{e^x - 1}{x}$$

$$x \neq 0 \quad \frac{e^x - 1}{x} \rightarrow \frac{0}{0}$$

$$x=0 \quad \frac{e^x - 1}{x} \rightarrow \frac{0}{0}$$

$$y = a \cos(\ln x) + b \sin(\ln x)$$

$$xy_1 = -a \sin(\ln x) + b \cos(\ln x)$$

$$x(xy_2 + y_1) = -a \cos(\ln x) - b \sin(\ln x) = -y$$

$$x^2 y_2 + xy_1 = -y$$

$$2xy_2 + x^2 y_3 + xy_2 + y_1 = -y_1$$

$$x^2 y_3 + 3xy_2 + 2y_1 = 0$$

$$y^{\frac{1}{m}} + y^{-\frac{1}{m}} = 2x$$

$$(x^2-1)y_3 + 3xy_2 + (1-m^2)y_1 = 0$$

$$t + \frac{1}{t} = 2x \Rightarrow t^2 - 2xt + 1 = 0, \quad t = x \pm \sqrt{x^2-1} = y^{\frac{1}{m}}$$

$$y = \left(x - \sqrt{x^2-1}\right)^m$$

$$y_1 = m \left(x - \sqrt{x^2-1}\right)^{m-1} \left(1 - \frac{x}{\sqrt{x^2-1}}\right) = \frac{-my}{\sqrt{x^2-1}}$$

$$(x^2-1)y_1^2 = m^2 y^2 \Rightarrow 2(x^2-1)y_1 y_2 + 2x y_1^2 = 2m^2 y y_1$$

$$(x^2-1)y_2 + x y_1 = m^2 y \Rightarrow (x^2-1)y_3 + 2x y_2 + x y_2 + y_1 = m^2 y_1$$

1. Use the substitution $x = \tan \theta$ to show that the equation

$$\frac{d^2 y}{dx^2} + \frac{2x}{1+x^2} \frac{dy}{dx} + \frac{y}{(1+x^2)^2} = 0$$

$$-\cancel{\sin 2\theta \cos^2 \theta \frac{dy}{d\theta}} + \cos^4 \theta \frac{d^2 y}{d\theta^2} + \cancel{\sin 2\theta \cos^3 \theta \frac{dy}{d\theta}} + y \cancel{\cos^4 \theta} \rightarrow \frac{dx}{d\theta} = \sec^2 \theta$$

$$= 0$$

$$\frac{dy}{dx} = \frac{dy}{d\theta} \frac{d\theta}{dx} = \cos^2 \theta \frac{dy}{d\theta}$$

$$\cos^4 \theta \left(\frac{d^2 y}{d\theta^2} + x \right) = 0$$

$$\frac{d^2 y}{dx^2} = \frac{d}{dx} \left(\cos^2 \theta \frac{dy}{d\theta} \right) = \frac{d}{d\theta} \left(\cos^2 \theta \frac{dy}{d\theta} \right) \frac{d\theta}{dx} = \cos^2 \theta \left(-\sin 2\theta \frac{dy}{d\theta} + \cos^2 \theta \frac{d^2 y}{d\theta^2} \right)$$

$$\frac{d^2 y}{dx^2} = -\sin 2\theta \cos^2 \theta \frac{dy}{d\theta} + \cos^4 \theta \frac{d^2 y}{d\theta^2}$$

2. P.T.

$$\frac{d^2x}{dy^2} = - \frac{\frac{d^2y}{dx^2}}{\left(\frac{dy}{dx}\right)^3} \Rightarrow \frac{d^3x}{dy^3} = - \frac{d}{dx} \left(\frac{\frac{d^2y}{dx^2}}{\left(\frac{dy}{dx}\right)^3} \right) \frac{dx}{dy}$$

$$\frac{3(y'')^2 - y' y'''}{(y')^5} = - \left(\frac{(y')^3 y''' - y'' 3(y')^2 y''}{(y')^6} \right) \frac{1}{y'}$$

$$\frac{dx}{dy} = \frac{1}{\left(\frac{dy}{dx}\right)}$$

$$= - \frac{1}{\left(\frac{dy}{dx}\right)^2} \frac{d^2y}{dx^2} \left(\frac{1}{\frac{dy}{dx}}\right) = \frac{- \frac{d^2y}{dx^2}}{\left(\frac{dy}{dx}\right)^3}$$

$$\frac{d^2x}{dy^2} = \frac{d}{dy} \left(\frac{1}{\frac{dy}{dx}} \right) = \frac{d}{dx} \left(\frac{1}{\left(\frac{dy}{dx}\right)} \right) \frac{dx}{dy}$$

$$= \frac{\left(\frac{dy}{dx}\right)(0) - 1 \left(\frac{d^2y}{dx^2}\right)}{\left(\frac{dy}{dx}\right)^2} \left(\frac{1}{\frac{dy}{dx}}\right)$$

Derivative of determinant

$$D(x) = \begin{vmatrix} f_1(x) & f_2(x) & f_3(x) \\ g_1(x) & g_2(x) & g_3(x) \\ h_1(x) & h_2(x) & h_3(x) \end{vmatrix} \quad D'(x) =$$

$$D'(x) = \begin{vmatrix} f_1'(x) & f_2'(x) & f_3'(x) \\ g_1(x) & g_2(x) & g_3(x) \\ h_1(x) & h_2(x) & h_3(x) \end{vmatrix} + \begin{vmatrix} f_1(x) & f_2(x) & f_3(x) \\ g_1'(x) & g_2'(x) & g_3'(x) \\ h_1(x) & h_2(x) & h_3(x) \end{vmatrix} + \begin{vmatrix} f_1(x) & f_2(x) & f_3(x) \\ g_1(x) & g_2(x) & g_3(x) \\ h_1'(x) & h_2'(x) & h_3'(x) \end{vmatrix}$$

$$\lim_{\Delta x \rightarrow 0} \frac{D(x+\Delta x) - D(x)}{\Delta x} =$$

$$\lim_{\Delta x \rightarrow 0} \frac{\begin{vmatrix} f_1(x+\Delta x) & f_2(x+\Delta x) & f_3(x+\Delta x) \\ g_1(x+\Delta x) & g_2(x+\Delta x) & g_3(x+\Delta x) \\ h_1(x+\Delta x) & h_2(x+\Delta x) & h_3(x+\Delta x) \end{vmatrix} - \begin{vmatrix} f_1(x) & f_2(x) & f_3(x) \\ g_1(x) & g_2(x) & g_3(x) \\ h_1(x) & h_2(x) & h_3(x) \end{vmatrix}}{\Delta x} =$$

$$\begin{vmatrix} f_1(x) & f_2(x) & f_3(x) \\ g_1(x) & g_2(x) & g_3(x) \\ h_1(x) & h_2(x) & h_3(x) \end{vmatrix} + \begin{vmatrix} f_1(x) & f_2(x) & f_3(x) \\ g_1(x) & g_2(x) & g_3(x) \\ h_1(x) & h_2(x) & h_3(x) \end{vmatrix} = \begin{vmatrix} f_1' & f_2' & f_3' \\ g_1 & g_2 & g_3 \\ h_1 & h_2 & h_3 \end{vmatrix} +$$

$$\lim_{\Delta x \rightarrow 0} \begin{vmatrix} f_1 & g_2 & h_3 \end{vmatrix} - \dots$$

PT-1 & PT-2